proof/lemma/chunks.v
@@ -1,75 +1,7 @@
 Require Import List Lia.
 Import ListNotations.
-From Minirust.def Require Import utils.
+From Minirust.def Require Import encoding utils.
 From Minirust.proof.lemma Require Import utils.
-
-Notation cstep l s := (
-  match firstn s l with
-  | [] => []
-  | x => x::(chunks (skipn s l) s)
-  end
-).
-
-Lemma skipn_smaller {T s} {l: list T} : length l >= length (skipn s l).
-Proof.
-generalize dependent s.
-induction l as [|x l IH].
-{ intros. destruct s; simpl; lia. }
-
-intros.
-simpl.
-destruct s. { simpl. lia. }
-simpl.
-have H (IH s).
-lia.
-Qed.
-
-Lemma waste_extra_gas {T s g1 g2} {l: list T} (H1: g1 >= length l) (H2: g2 >= length l):
-  chunks_impl g1 l (S s) = chunks_impl g2 l (S s).
-Proof.
-generalize dependent g2.
-generalize dependent l.
-
-induction g1 as [|g1 IH].
-{ intros. destruct l; try simpl in H1; try lia; destruct g2; simpl; auto. }
-
-intros.
-destruct l.
-{ simpl. destruct g2; simpl; auto. }
-
-destruct g2.
-{ simpl in H2. lia. }
-
-simpl.
-f_equal.
-assert (length (skipn s l) <= length l). { apply skipn_smaller. }
-
-assert (g1 >= length l).
-{ simpl in H1. lia. }
-
-assert (g2 >= length l).
-{ simpl in H2. lia. }
-
-apply IH; lia.
-Qed.
-
-Lemma chunks_step {T s} {l: list T} : chunks l s = cstep l s.
-Proof.
-(* first, finish the s = 0 case, where no iteration happens at all *)
-destruct s.
-{ unfold chunks. simpl. destruct l; simpl; auto. }
-
-unfold chunks.
-
-induction l as [| x l IH].
-{ unfold chunks. auto. }
-
-simpl.
-f_equal.
-refine (waste_extra_gas _ _).
-- apply skipn_smaller.
-- lia.
-Qed.
 
 Lemma concat_len {T n k} {ll: list (list T)}
   (Hl1: length ll = k)
@@ -108,13 +40,12 @@ rewrite app_length.
 lia.
 Qed.
 
-Lemma chunks_len {T n k} {l: list T} (H: length l = n * k) :
-  length (chunks l n) = k /\ Forall (fun x => length x = n) (chunks l n).
+Lemma chunks_len {T c s} {l: list T} (H: length l = c * s) :
+  length (chunks c s l) = c /\ Forall (fun x => length x = s) (chunks c s l).
 Proof.
 Admitted.
 
-
-Lemma chunks_concat {T} {s} {l : list (list T)} (H: Forall (fun x => length x = s) l) :
-  chunks (concat l) s = l.
+Lemma chunks_concat {T c s} {l : list (list T)} (H1: length l = c) (H: Forall (fun x => length x = s) l) :
+  chunks c s (concat l) = l.
 Proof.
 Admitted.
